%!Mode:: "TeX:UTF-8"
%!TEX encoding = UTF-8 Unicode
%!TEX TS-program = xelatex
\documentclass{ctexart}
\newif\ifpreface
%\prefacetrue
\input{../../../global/all}
\begin{document}
\large
\setlength{\baselineskip}{1.2em}
\ifpreface
    \input{../../../global/preface}
\else
%\maketitle
\fi
\newgeometry{left=2cm,right=2cm,top=2cm,bottom=2cm}
%from_here_to_type
\begin{problem}\label{pro:1}
  \begin{enumerate}
    \item   Assume \(\{Y_i(n):n \geq 0\}, \{Y_2(n):n \geq 0\}\) are two independent migrating branch process with descending distribution 
  \((p(i):i \in \mathbb{Z}_+)\) and the migrating probobility respectively are \((\gamma_1(i): i \in \mathbb{Z}_{+}),(\gamma_2(i): i \in \mathbb{Z}_+)\). 
  Prove: \(\{Y_1(n )+ Y_2(n): n \geq 0\}\) is migrating branching process with descending distribution \(p(i): i \in \mathbb{Z}_+\) 
  and migrating probability \(\gamma_1 * \gamma_2(i): i \in \mathbb{Z}_+\).
\item   Let \(\{Y(n): n \in \mathbb{Z}_+\}\) be migrating branch process with descending distribution \(p(j): j \in \mathbb{Z}_+\)
  and the migrating distribution \(\gamma(i): i \in \mathbb{Z}_+\). 
  \(P_n^\gamma=(p_n^\gamma (i,j); i,j \in \mathbb{Z}_+)\) is the \(n\)-th transition matrix. 
  Prove: \(\forall i,n \geq 1\)
  \[
    \sum_{j=0}^{\infty} p_n^\gamma(i,j)z^j = g_n(z)^i \prod_{k=1}^{n} h(g_{k-1}(z)), |z| \leq 1
  \]
  where \(h\) is the generating function of \((\gamma(j): j \in \mathbb{Z}_+)\).
  \(g\) is the generating funtion of \((p(j): j \in \mathbb{Z}_+)\).
\item  \(h,g\) are defined as above. Assume \(m :=g'(1-) < \infty, \mu:=h'(1-) < \infty\). 
  Prove: \(\forall i,n \geq 1\), \[
    \mathbb{P}(Y_n \mid Y_0 =i)=im^n + \mu \sum_{k=1}^{n} m^{k-1}
  \]
  \end{enumerate}
\end{problem}
\begin{problem}\label{pro:2}
  Assume \(b \in (0,1), p \in (0,1)\). Let \(\mu(0)=\frac{1-b-p}{1-p}\mu(j)=bp^{j-1},j \geq 1\). 
  Prove: 
\begin{enumerate}
  \item   \((\mu(j):j \in \mathbb{Z}_+)\) is probability distribution and \[
    g(z):=\sum_{j=0}^{\infty} \mu(j)z^j=\frac{1-b-p}{1-p} + \frac{bz}{1-pz}.
  \]

\item Let \(b =(1-p)^2\). 
  Prove: 
\begin{enumerate}
  \item   \(g'(1)=1\) and \[
    g(z)=p + \frac{(1-p)^2 z}{1-pz}=\frac{p-(2p-1)z}{1-pz}.
  \]
\item \(\forall n \geq 1\), then \[
  g_n(z)=\frac{np-((n + 1)p-1)z}{1 + (n-1)p-npz}.
\]     
\end{enumerate}
\end{enumerate}
\end{problem}
\begin{problem}\label{pro:3}

  
\end{problem}




\end{document}
